\documentclass[12pt]{article}

\input{packages.tex}
\input{style.tex}

\begin{document}

\title{Matrices and Matrix Operations}
\author{Brian D.\ Fitzpatrick}
\date{\cite[\S1.2]{peterson}}

\maketitle

% \tableofcontents

\begin{sagesilent}
  latex.matrix_delimiters(left='[', right=']')
\end{sagesilent}

\begin{definition}
  A \emph{matrix of size $m\times n$} is an object of the form
  \begin{align*}
    A &= 
    \begin{bmatrix}
      a_{11} & a_{12} & \dotsb & a_{1n} \\
      a_{21} & a_{22} & \dotsb & a_{2n} \\
      \vdots & \vdots & \ddots & \vdots \\
      a_{m1} & a_{m2} & \dotsb & a_{mn}
    \end{bmatrix} &
    \underbrace{m}_{\#\mathtt{rows}}\times\underbrace{n}_{\#\mathtt{columns}}
  \end{align*}
  where $a_{ij}\in\RR$. 
\end{definition}

\begin{sagesilent}
  A = matrix([[2,0],[4,1],[16,-3/4]])
  B = matrix([[3,0,8,1,2],[7,-1/2,3,2,10],[32,1,0,0,0]])
\end{sagesilent}

\begin{ex}
  \begin{align*}
    A &= \sage{A} & 3\times 2 && a_{21} &= 4 \\
    B &= \sage{B} & 3\times 5 && b_{32} &= 1 
  \end{align*}
\end{ex}

\begin{notation}
  The entries of $A=[a_{ij}]$ are often denoted by
  \[
  a_{ij}=[A]_{ij}=\ent_{ij}(A)
  \]
\end{notation}

\begin{definition}
  The collection of all $m\times n$ matrices is denoted by $M_{m\times n}(\RR)$.
\end{definition}

\begin{definition}
  Matrices in $M_{1\times n}(\RR)$ are called \emph{row vectors}. Matrices in
  $M_{m\times 1}(\RR)$ are called \emph{column vectors}.
\end{definition}

\begin{ex}
  We have the identifications
  \begin{align*}
    M_{2\times 2}(\RR) &=
    \Set*{
      \begin{bmatrix}
        a_{11} & a_{12} \\
        a_{21} & a_{22}
      \end{bmatrix}\given a_{ij}\in\RR} &
    \RR^n &= M_{n\times 1} = 
    \Set*{
      \begin{bmatrix}
        a_1\\ a_2\\ \vdots \\ a_n
      \end{bmatrix}
      \given a_i\in\RR
    }
  \end{align*}
\end{ex}

\section{Matrix Addition}

\begin{definition}
  The \emph{sum} of two $m\times n$ matrices $A$ and $B$ is the $m\times n$
  matrix $A+B$ whose entries are $[A+B]_{ij}=a_{ij}+b_{ij}$.
\end{definition}

\begin{sagesilent}
  A = matrix([[3,1,8],[2,4,-1]])
  B = matrix([[0,-3,-4],[1,2,-7]])
\end{sagesilent}

\begin{ex}
  $\sage{A}+\sage{B}=\sage{A+B}$
\end{ex}

\begin{note}
  $A+B$ is only defined when $A$ and $B$ \emph{have the same size}
\end{note}

\section{Scalar Multiplication}

\begin{definition}
  The \emph{scalar product} of $\lambda\in\RR$ and $A\in M_{m\times n}(\RR)$ is
  the $m\times n$ matrix $\lambda A$ whose entries are $[\lambda A]_{ij}=\lambda
  a_{ij}$.
\end{definition}

\begin{ex}
  $6\sage{A}=\sage{6*A}$
\end{ex}

\begin{samepage}
  \begin{thm}[Theorem 1.2 in \cite{peterson}]
    Let $A,B,C\in M_{m\times n}(\RR)$ and let $\alpha,\beta\in\RR$. Then
    \begin{enumerate}
    \item $A+B=B+A$
    \item $A+(B+C)=(A+B)+C$
    \item $\alpha(\beta A)=(\alpha\beta)A$
    \item $\alpha(A+B)=\alpha A+\alpha B$
    \item $(\alpha+\beta)A=\alpha A+\beta A$
    \end{enumerate}
  \end{thm}
\end{samepage}

\begin{definition}
  The \emph{$m\times n$ zero matrix} is the $m\times n$ matrix $0_{m\times n}$
  whose entries are $[0_{m\times n}]_{ij}=0$.
\end{definition}

\begin{ex}
  $0_{3\times 4}=\sage{zero_matrix(3,4)}$
\end{ex}

\begin{thm}
  Let $A\in M_{m\times n}(\RR)$. Then
  \begin{enumerate}
  \item $A+0_{m\times n}=A$
  \item $0\cdot A=0_{m\times n}$
  \item $A-A=0_{m\times n}$
  \end{enumerate}
\end{thm}

\section{Matrix Multiplication}

\begin{definition}
  Let $A\in M_{l\times m}(\RR)$ and $B\in M_{m\times n}(\RR)$. The
  \emph{product} of $A$ and $B$ is the $l\times n$ matrix $AB$ whose entries are
  \[
  [AB]_{ij}=\sum_{k=1}^m a_{ik}b_{kj}
  \]
\end{definition}

\begin{note}
  The product $AB$ is only defined when
  \[
  \#\texttt{ columns of } A = \#\texttt{ rows of }B
  \]
\end{note}

\begin{idea}
  The $(i,j)$ entry of $AB$ is given by the dot-product
  \begin{align*}
    [AB]_{ij}
    &= (i^{\texttt{th}}\texttt{ row of }A)\cdot(j^{\texttt{th}}\texttt{ column of }B) \\
    &= 
    \begin{bmatrix}
      \\ a_{i1} & a_{i2} & \dotsb & a_{in} \\ \\
    \end{bmatrix}
    \begin{bmatrix}
      && b_{1j} && \\
      && b_{2j} && \\
      && \vdots && \\
      && b_{mj} && 
    \end{bmatrix}
  \end{align*}
\end{idea}

\begin{sagesilent}
  A = matrix([[3,4],[1,-8]])
  B = matrix([[1,0],[2,0],[3,1]])
\end{sagesilent}

\begin{ex}
  Find $AB$ and $BA$ where
  \begin{align*}
    A &= \sage{A} & B &= \sage{B}
  \end{align*}
\end{ex}
\begin{sol}
  Note that $A$ is $2\times 2$ and $B$ is $3\times 2$. Since $2\neq 3$, $AB$ is
  not defined.

  However, $BA$ is defined and
  \[
  BA=\sage{B}\sage{A}=\sage{B*A}
  \]
\end{sol}

\begin{samepage}
  \begin{thm}[Theorem 1.3 in \cite{peterson}]
    Let $A$, $B$, and $C$ be matrices and let $\lambda\in\RR$. Then
    \begin{enumerate}
    \item $A(BC)=(AB)C$
    \item $A(B+C)=AB+AC$
    \item $(A+B)C=AC+BC$
    \item $\lambda(AB)=(\lambda A)B=A(\lambda B)$
    \end{enumerate}
  \end{thm}
\end{samepage}

\begin{definition}
  The \emph{$n\times n$ identity matrix} is the $n\times n$ matrix $I_n$ whose
  entries are
  \[
  [I_n]_{ij} =
  \delta_{ij}=
  \begin{cases}
    1 & i=j \\
    0 & i\neq j
  \end{cases}
  \]
\end{definition}

\begin{ex}
  \begin{align*}
    I_2 &= \sage{identity_matrix(2)} &
    I_3 &= \sage{identity_matrix(3)} &
    I_4 &= \sage{identity_matrix(4)} 
  \end{align*}
\end{ex}

\begin{samepage}
  \begin{thm}
    Let $A\in M_{m\times n}(\RR)$. Then
    \begin{enumerate}
    \item $0_{l\times m}A=0_{l\times n}$ and $A0_{n\times l}=0_{m\times l}$
    \item $I_mA=AI_n=A$
    \end{enumerate}
  \end{thm}
  \begin{proof}
    To prove that $I_mA=A$, note that
    \[
    [I_mA]_{ij}=\sum_{k=1}^m[I_m]_{ik}a_{kj}=\sum_{k=1}^m\delta_{ik}a_{kj}=a_{ij}
    \]
    Proving that $AI_n=A$ is similar.
  \end{proof}
\end{samepage}

The previous two theorems show that matrix arithmetic is similar to ''usual''
arithmetic. However, there are some key differences.

\begin{sagesilent}
  A = matrix([[0,1],[0,0]])
  B = matrix([[1,0],[0,0]])
\end{sagesilent}

\begin{ex}
  Find $AB$ and $BA$ where
  \begin{align*}
    A &= \sage{A} &
    B &= \sage{B}
  \end{align*}
\end{ex}
\begin{sol}
  Compute
  \begin{align*}
    AB &= \sage{A}\sage{B}=\sage{A*B} &
    BA &= \sage{B}\sage{A}=\sage{B*A}
  \end{align*}
  So $AB\neq BA$. Furthermore, $AB=0_{2\times 2}$ even though $A\neq 0_{w\times
    2}$ and $B\neq0_{2\times 2}$.
\end{sol}

\section{Motivation}

The system
\[
\begin{array}{rcrcccrcr}
  a_{11}x_1 & + & a_{12}x_2 & + & \dotsb & + & a_{1n}x_n & = & b_1 \\
  a_{21}x_1 & + & a_{22}x_2 & + & \dotsb & + & a_{2n}x_n & = & b_2 \\
  \vdots   &   & \vdots   &   & \ddots &   & \vdots   &   & \vdots \\
  a_{m1}x_1 & + & a_{m2}x_2 & + & \dotsb & + & a_{mn}x_n & = & b_m \\
\end{array}
\]
may be written as $A\vec x=\vec b$ where
\begin{align*}
  A &= 
  \begin{bmatrix}
    a_{11} & a_{12} & \dotsb & a_{1n} \\
    a_{21} & a_{22} & \dotsb & a_{2n} \\
    \vdots & \vdots & \ddots & \vdots \\
    a_{m1} & a_{m2} & \dotsb & a_{mn}
  \end{bmatrix} &
  \vec x &=
  \begin{bmatrix}
    x_1\\ x_2\\ \vdots\\ x_n
  \end{bmatrix} &
  \vec b &=     
  \begin{bmatrix}
    b_1\\ b_2\\ \vdots\\ b_m
  \end{bmatrix}
\end{align*}

\begin{sagesilent}
  A = matrix([[2,-1,4],[1,-7,1],[-1,2,1]])
  var('x y z')
  vx = matrix([[x, y, z]]).transpose()
  b = matrix([[1,3,2]]).transpose()
\end{sagesilent}

\begin{ex}
  The system
  \[
  \begin{array}{rcrcrcr}
    2\,x & - & y    & + & 4\,z & = & 1 \\
    x & - & 7\,y & + &    z & = & 3 \\
    -x & + & 2\,y & + &    z & = & 2
  \end{array}
  \]
  may be written as
  \[
  \sage{A}\sage{vx}=\sage{b}
  \]
\end{ex}

\bibliography{mybib.bib}{}
\bibliographystyle{plain}

\end{document}
