\documentclass[12pt]{article}

\input{packages.tex}
\input{style.tex}

\begin{document}

\title{Determinants}
\author{Brian D.\ Fitzpatrick}
\date{\cite[\S1.5]{peterson}}

\maketitle

% \tableofcontents

\begin{sagesilent}
  latex.matrix_delimiters(left='[', right=']')
\end{sagesilent}

\begin{definition}
  The \emph{$(i,j)$-submatrix} of a $n\times n$ matrix $A$ is the
  $(n-1)\times(n-1)$ matrix obtained by deleting the $i$th row and $j$th column
  of $A$. We denote the $(i,j)$-submatrix of $A$ by $A_{ij}$.
\end{definition}

\begin{sagesilent}
  A = matrix([[1,2,3],[7,0,10],[0,-1,6]])
  A21 = matrix([[2,3],[-1,6]])
\end{sagesilent}
\begin{ex}
  $A = \sage{A}\implies A_{21} = \sage{A21}$
\end{ex}


\begin{definition}
  The \emph{determinant} of a $1\times 1$ matrix $A=[a_{11}]$ is
  $\det(A)=a_{11}$.
\end{definition}

\begin{definition}
  The \emph{determinant} of a $n\times n$ matrix $A$ is
  $\displaystyle\det(A)=\sum_{k=1}^n(-1)^{1+k}a_{1k}\det(A_{1k})$
\end{definition}

\begin{note}
  We often write $\det(A)=\abs{A}$.
\end{note}

\begin{sagesilent}
  var('a b c d')
  A = matrix([[a,b],[c,d]])
\end{sagesilent}
\begin{ex}
  Compute $\det\sage{A}$.
\end{ex}
\begin{sol}\leavevmode
  \begin{align*}
    \det(A) 
    &= \sum_{k=1}^2(-1)^{1+k}a_{1k}\det(A_{1k}) \\
    &= (-1)^{1+1}a_{11}\det(A_{11})+(-1)^{1+2}a_{12}\det(A_{12}) \\
    &= a\det([d])-b\det([c]) \\
    &= ad-bc
  \end{align*}
\end{sol}


\newpage
\begin{sagesilent}
  var('a11 a12 a13 a21 a22 a23 a31 a32 a33')
  A = matrix([[a11, a12, a13],[a21, a22, a23],[a31, a32, a33]])
\end{sagesilent}
\begin{ex}
  Compute $\det\sage{A}$.
\end{ex}
\begin{sagesilent}
  latex.matrix_delimiters(left='|', right='|')
  M = lambda i,j: A.delete_rows([i-1]).delete_columns([j-1])
\end{sagesilent}
\begin{sol}\leavevmode
  \begin{align*}
    \det(A)
    &= \sum_{k=1}^3(-1)^{1+k}a_{1k}\det(A_{1k}) \\
    &= (-1)^{1+1}a_{11}\det(A_{11})+(-1)^{1+2}a_{12}+(-1)^{1+3}a_{13}\det(A_{13}) \\
    &= a_{11}\sage{M(1,1)}-a_{12}\sage{M(1,2)}+a_{13}\sage{M(1,3)}
  \end{align*}
\end{sol}


\newpage
\begin{definition}
  The \emph{$(i,j)$-minor} of $A$ is $M_{ij}=\det(A_{ij})$. The
  \emph{$(i,j)$-cofactor} of $A$ is $C_{ij}=(-1)^{i+j}M_{ij}$.
\end{definition}

\begin{note}
  We this notation, our formula for determinants is
  \[
  \det(A)=\sum_{k=1}^n a_{1k}C_{1k}
  \]
\end{note}
\begin{sagesilent}
  latex.matrix_delimiters(left='[', right=']')
  var('a11 a12 a13 a21 a22 a23 a31 a32 a33')
  A = matrix([[a11, a12, a13],[a21, a22, a23],[a31, a32, a33]])
\end{sagesilent}
\begin{ex}
  For $A=\sage{A}$ we have%
  \begin{sagesilent}
    latex.matrix_delimiters(left='|', right='|')
    M = lambda i,j: A.delete_rows([i-1]).delete_columns([j-1])
  \end{sagesilent}%
  \begin{align*}
    C_{11} &= (-1)^{1+1}\sage{M(1,1)} =  \sage{M(1,1)} \\
    C_{12} &= (-1)^{1+2}\sage{M(1,2)} = -\sage{M(1,2)} \\
    C_{32} &= (-1)^{3+2}\sage{M(3,2)} = -\sage{M(3,2)}
  \end{align*}
\end{ex}

\newpage
\begin{note}
  The signs of the cofactors can be remembered by
  \[
  \begin{matrix}
    + & - & + & - & \cdots \\
    - & + & - & + & \cdots \\
    + & - & + & - & \cdots \\
    \vdots & \vdots & \vdots & \vdots & \ddots
  \end{matrix}
  \]
\end{note}


\begin{thm}[Laplace Cofactor Expansion Theorem, Theorem 1.16 in \cite{peterson}]
  For any $1\leq i\leq n$ we have
  \begin{align*}
    \det(A) &= \sum_{k=1}^n a_{ik}C_{ik}\tag{$i$th row expansion} \\
    \det(A) &= \sum_{k=1}^n a_{ki}C_{ki}\tag{$i$th column expansion} 
  \end{align*}
\end{thm}

\begin{idea}
  The Laplace Cofactor Expansion Theorem allows us to compute determinants by
  ``expanding'' about any row or column. This is nice because some rows or
  columns may be easier to expand about than others.
\end{idea}

\newpage

\begin{sagesilent}
  latex.matrix_delimiters(left='|', right='|')
  A = matrix([[1,2,3],[4,5,6],[7,8,9]])
  M = lambda i,j: A.delete_rows([i-1]).delete_columns([j-1])
\end{sagesilent}
\begin{ex}
  Compute $\sage{A}$.
\end{ex}
\begin{sol}
  Expansion about $\Row_2$ gives
  \[
  \sage{A}
  =(\sage{(-1)**(2+1)*A[1,0]})\sage{M(2,1)}
  +(\sage{(-1)**(2+2)*A[1,1]})\sage{M(2,2)}
  +(\sage{(-1)**(2+3)*A[1,2]})\sage{M(2,3)}
  =\sage{A.det()}
  \]
  Expansion about $\Col_3$ gives
  \[
  \sage{A}
  =(\sage{(-1)**(1+3)*A[0,2]})\sage{M(1,3)}
  +(\sage{(-1)**(2+3)*A[1,2]})\sage{M(2,3)}
  +(\sage{(-1)**(3+3)*A[2,2]})\sage{M(3,3)}
  =\sage{A.det()}
  \]
\end{sol}

\newpage
\begin{sagesilent}
  latex.matrix_delimiters(left='|', right='|')
  A = matrix([[7,-3,0,4],[0,1,0,3],[2,1,-2,-5],[0,4,0,6]])
  M = lambda X, i,j: X.delete_rows([i-1]).delete_columns([j-1])
\end{sagesilent}
\begin{ex}
  Compute $\sage{A}$.
\end{ex}
\begin{sol}
  Expansion about $\Col_3$ gives
  \[
  \sage{A}=(-2)\sage{M(A, 3, 3)}
  \]
  Then expand about $\Col_1$ to obtain
  \[
  \sage{M(A, 3, 3)} = (7)\sage{M(M(A, 3, 3), 1, 1)} = 7(6-12) = -42
  \]
  Hence
  \[
  \sage{A}=(-2)(-42)=\sage{A.det()}
  \]
\end{sol}


\newpage
\begin{thm}[Corollary 1.17 in \cite{peterson}]
  If $A$ has a row or column of zeros, then $\det(A)=0$.
\end{thm}

\begin{thm}[Corollary 1.18 in \cite{peterson}]
  The determinant of a triangular matrix is the product of its diagonal entries.
\end{thm}

\begin{thm}[Theorem 1.19 in \cite{peterson}]
  $\det(A^\top)=\det(A)$
\end{thm}

\begin{thm}[Theorem 1.20 in \cite{peterson}]\leavevmode
  \begin{enumerate}
  \item $A\xrightarrow{R_i\leftrightarrow R_j}B\implies\det(B)=-\det(A)$
  \item $A\xrightarrow{\lambda R_i\to R_i}B\implies\det(B)=\lambda\det(A)$
  \item $A\xrightarrow{R_i+\lambda R_j\to R_i}B\implies\det(B)=\det(A)$
  \end{enumerate}
\end{thm}

\begin{idea}
  Determinants play nicely with elementary row operations.
\end{idea}


\bibliography{mybib.bib}{}
\bibliographystyle{plain}

\end{document}
